src/n-bit/wordsScript.sml
@@ -34,34 +34,24 @@ val HB = ``^WL - 1``;
 
 val _ = ai := false;
 
-val TOP_def = Define `TOP (:'a) = 2 ** ^WL`
-val TOP = save_thm("TOP", TOP_def)
-val TOP_ML = rhs (#2 (strip_forall (concl TOP)))
+val dimword_def  = Define `dimword (:'a) = 2 ** ^WL`
+val INT_MIN_def  = Define `INT_MIN (:'a) = 2 ** ^HB`
 
-val ZERO_LT_TOP = store_thm(
-  "ZERO_LT_TOP",
-  `0 < TOP(:'a)`,
-  SRW_TAC [][TOP])
-val _ = export_rewrites ["ZERO_LT_TOP"]
+val _ = ai := true;
 
-val MSB_def = Define `MSB (:'a) = 2 ** ^HB`
-val MSB = save_thm("MSB", MSB_def)
-val MSB_ML = rhs (#2 (strip_forall (concl MSB)))
+val UINT_MAX_def = Define `UINT_MAX (:'a) = dimword(:'a) - 1`;
+val INT_MAX_def  = Define `INT_MAX (:'a) = INT_MIN(:'a) - 1`;
 
-val TOP_IS_TWICE_MSB = store_thm(
-  "TOP_IS_TWICE_MSB",
-  `TOP(:'a) = 2 * MSB(:'a)`,
-  SRW_TAC [][TOP,MSB] THEN
-  `0 < dimindex (:'a)` by (ASSUME_TAC DIMINDEX_GE_1 THEN DECIDE_TAC) THEN
-  Cases_on `dimindex(:'a)` THEN1 FULL_SIMP_TAC (srw_ss()) [] THEN
-  SRW_TAC [][EXP]);
-
+val dimword_ML = rhs (#2 (strip_forall (concl dimword_def)))
+val INT_MIN_ML = rhs (#2 (strip_forall (concl INT_MIN_def)))
 
 val _ = type_abbrev("word", ``:bool ** 'a``);
 
 (* ------------------------------------------------------------------------- *)
 (*  Domain transforming maps : definitions                                   *)
 (* ------------------------------------------------------------------------- *)
+
+val _ = ai := false;
 
 val w2n_def = Define`
   w2n (w:'a word) = SUM ^WL (\i. SBIT (w %% i) i)`;
@@ -85,13 +75,13 @@ val _ = add_bare_numeral_form (#"w", SOME "n2w");
 (* ------------------------------------------------------------------------- *)
 
 val word_T_def = Define`
-  word_T = n2w:num->('a word) (TOP(:'a) - 1)`;
+  word_T = n2w:num->('a word) (UINT_MAX(:'a))`;
 
 val word_L_def = Define`
-  word_L = n2w:num->('a word) (MSB(:'a))`;
+  word_L = n2w:num->('a word) (INT_MIN(:'a))`;
 
 val word_H_def = Define`
-  word_H = n2w:num->('a word) (MSB(:'a) - 1)`;
+  word_H = n2w:num->('a word) (INT_MAX(:'a))`;
 
 val _ = ai := false;
 
@@ -116,6 +106,9 @@ val _ = overload_on ("&&",Term`$word_and`);
 val _ = overload_on ("!!",Term`$word_or`);
 val _ = overload_on ("??",Term`$word_xor`);
 val _ = overload_on ("Tw",Term`word_T`);
+val _ = overload_on ("UINT_MAXw",Term`word_T`);
+val _ = overload_on ("INT_MAXw",Term`word_H`);
+val _ = overload_on ("INT_MINw",Term`word_L`);
 
 val _ = add_infix("&&",400,HOLgrammars.RIGHT);
 val _ = add_infix("!!",300,HOLgrammars.RIGHT);
@@ -172,7 +165,7 @@ val _ = add_infix("><",350,HOLgrammars.RIGHT);
 
 val word_2comp_def = Define`
   word_2comp (w:'a word) =
-    n2w:num->('a word) (TOP(:'a) - w2n w)`;
+    n2w:num->('a word) (dimword(:'a) - w2n w)`;
 
 val word_add_def = Define`
   word_add (v:'a word) (w:'a word) =
@@ -337,6 +330,20 @@ val _ = add_infix(">=+",450,HOLgrammars.RIGHT);
 (*  Theorems                                                                 *)
 (* ------------------------------------------------------------------------- *)
 
+val ZERO_LT_dimword = store_thm(
+  "ZERO_LT_dimword",
+  `0 < dimword(:'a)`,
+  SRW_TAC [][dimword_def])
+val _ = export_rewrites ["ZERO_LT_dimword"]
+
+val dimword_IS_TWICE_INT_MIN = store_thm(
+  "dimword_IS_TWICE_INT_MIN",
+  `dimword(:'a) = 2 * INT_MIN(:'a)`,
+  SRW_TAC [][dimword_def,INT_MIN_def] THEN
+  `0 < dimindex (:'a)` by (ASSUME_TAC DIMINDEX_GE_1 THEN DECIDE_TAC) THEN
+  Cases_on `dimindex(:'a)` THEN1 FULL_SIMP_TAC (srw_ss()) [] THEN
+  SRW_TAC [][EXP]);
+
 val DIMINDEX_GT_0 = save_thm("DIMINDEX_GT_0",
   PROVE [DECIDE ``!s. 1 <= s ==> 0 < s``,DIMINDEX_GE_1] ``0 < dimindex(:'a)``);
 
@@ -348,8 +355,8 @@ val EXISTS_HB = save_thm("EXISTS_HB",
   PROVE [DIMINDEX_GT_0,LESS_ADD_1,ADD1,ADD] ``?m. ^WL = SUC m``);
 
 val MOD_DIMINDEX = store_thm("MOD_DIMINDEX",
-  `!n. n MOD TOP (:'a) = BITS (^WL - 1) 0 n`,
-  STRIP_ASSUME_TAC EXISTS_HB \\ ASM_SIMP_TAC arith_ss [TOP_def,BITS_ZERO3]);
+  `!n. n MOD dimword (:'a) = BITS (^WL - 1) 0 n`,
+  STRIP_ASSUME_TAC EXISTS_HB \\ ASM_SIMP_TAC arith_ss [dimword_def,BITS_ZERO3]);
 
 val SUB1_SUC = DECIDE (Term `!n. 0 < n ==> (SUC (n - 1) = n)`);
 val SUB_SUC1 = DECIDE (Term `!n. ~(n = 0) ==> (SUC (n - 1) = n)`);
@@ -381,8 +388,8 @@ val w2n_n2w_lem = prove(
     \\ RW_TAC (fcp_ss++ARITH_ss) [BIT_SLICE_THM]);
 
 val w2n_n2w = store_thm("w2n_n2w",
-  `!n. w2n (n2w:num->('a word) n) = n MOD (TOP(:'a))`,
-  SIMP_TAC (fcp_ss++WORD_ss) [w2n_n2w_lem,SUM_SLICE, TOP]);
+  `!n. w2n (n2w:num->('a word) n) = n MOD (dimword(:'a))`,
+  SIMP_TAC (fcp_ss++WORD_ss) [w2n_n2w_lem,SUM_SLICE, dimword_def]);
 val _ = export_rewrites ["w2n_n2w"]
 
 val n2w_w2n_lem = prove(
@@ -422,29 +429,29 @@ fun Cases_word (g as (_,w)) =
   end
 
 val n2w_mod = store_thm("n2w_mod",
-  `!n. n2w:num -> 'a word (n MOD TOP(:'a)) = n2w n`,
-  RW_TAC fcp_ss [TOP]
+  `!n. n2w:num -> 'a word (n MOD dimword(:'a)) = n2w n`,
+  RW_TAC fcp_ss [dimword_def]
     \\ STRIP_ASSUME_TAC EXISTS_HB
     \\ ASM_SIMP_TAC (fcp_ss++ARITH_ss)
          [n2w_def,MIN_DEF,BIT_def,GSYM BITS_ZERO3,BITS_COMP_THM2]);
 
 val n2w_11 = store_thm("n2w_11",
-  `!m n. ((n2w m):bool **'a = n2w n) = (m MOD TOP(:'a) = n MOD TOP(:'a))`,
+  `!m n. ((n2w m):bool **'a = n2w n) = (m MOD dimword(:'a) = n MOD dimword(:'a))`,
   NTAC 2 STRIP_TAC
     \\ STRIP_ASSUME_TAC EXISTS_HB
-    \\ ASM_SIMP_TAC (fcp_ss++WORD_ss) [GSYM BITS_ZERO3,TOP]
+    \\ ASM_SIMP_TAC (fcp_ss++WORD_ss) [GSYM BITS_ZERO3,dimword_def]
     \\ EQ_TAC \\ RW_TAC arith_ss [DECIDE ``i < SUC p = i <= p``]
     \\ PROVE_TAC [(REWRITE_RULE [ZERO_LESS_EQ] o SPECL [`p`,`0`]) BIT_BITS_THM]
 );
 val _ = export_rewrites ["n2w_11"]
 
 val ranged_word_nchotomy = store_thm("ranged_word_nchotomy",
-  `!w : bool ** 'a. ?n. (w = n2w n) /\ n < TOP(:'a)`,
+  `!w : bool ** 'a. ?n. (w = n2w n) /\ n < dimword(:'a)`,
   STRIP_TAC
     \\ Q.ISPEC_THEN `w` STRUCT_CASES_TAC word_nchotomy
     \\ SIMP_TAC (srw_ss()) [n2w_11]
-    \\ Q.EXISTS_TAC `n MOD TOP(:'a)`
-    \\ SIMP_TAC (srw_ss()) [TOP, MOD_MOD, DIVISION])
+    \\ Q.EXISTS_TAC `n MOD dimword(:'a)`
+    \\ SIMP_TAC (srw_ss()) [dimword_def, MOD_MOD, DIVISION])
 
 val w2n_11 = store_thm("w2n_11",
   `!v w. (w2n v = w2n w) = (v = w)`,
@@ -453,11 +460,11 @@ val w2n_11 = store_thm("w2n_11",
 val _ = export_rewrites ["w2n_11"]
 
 val w2n_lt = store_thm("w2n_lt",
-  `!w:'a word. w2n w < TOP(:'a)`,
-  SIMP_TAC std_ss [w2n_def,SUM_SBIT_LT,TOP]);
+  `!w:'a word. w2n w < dimword(:'a)`,
+  SIMP_TAC std_ss [w2n_def,SUM_SBIT_LT,dimword_def]);
 
 val word_0_n2w = store_thm("word_0_n2w",
-  `w2n 0w = 0`, SIMP_TAC arith_ss [w2n_n2w, ZERO_LT_TOP]);
+  `w2n 0w = 0`, SIMP_TAC arith_ss [w2n_n2w, ZERO_LT_dimword]);
 
 val w2n_eq_0 = store_thm("w2n_eq_0",
   `(w2n w = 0) = (w = 0w)`,
@@ -467,15 +474,15 @@ val _ = export_rewrites ["w2n_eq_0"]
 val word_add_n2w = store_thm("word_add_n2w",
   `!m n. n2w m + n2w n = n2w (m + n)`,
   SIMP_TAC fcp_ss [word_add_def,w2n_n2w] \\ ONCE_REWRITE_TAC [GSYM n2w_mod]
-    \\ SIMP_TAC arith_ss [MOD_PLUS, ZERO_LT_TOP]);
+    \\ SIMP_TAC arith_ss [MOD_PLUS, ZERO_LT_dimword]);
 
 val word_mul_n2w = store_thm("word_mul_n2w",
   `!m n. n2w m * n2w n = n2w (m * n)`,
   SIMP_TAC fcp_ss [word_mul_def,w2n_n2w] \\ ONCE_REWRITE_TAC [GSYM n2w_mod]
-    \\ SIMP_TAC arith_ss [MOD_TIMES2,ZERO_LT_TOP]);
+    \\ SIMP_TAC arith_ss [MOD_TIMES2,ZERO_LT_dimword]);
 
 val word_log2_n2w = store_thm("word_log2_n2w",
-  `!n. word_log2 (n2w n):'a word = n2w (LOG2 (n MOD TOP(:'a)))`,
+  `!n. word_log2 (n2w n):'a word = n2w (LOG2 (n MOD dimword(:'a)))`,
   SIMP_TAC fcp_ss [word_log2_def,w2n_n2w]);
 
 val top = ``2 ** wl``;
@@ -494,11 +501,11 @@ val ONE_COMP_THM = prove(
     \\ ASM_SIMP_TAC bool_ss [BITWISE_THM]);
 
 val word_1comp_n2w = store_thm("word_1comp_n2w",
-  `!n. ~(n2w n):'a word  = n2w (TOP(:'a) - 1 - n MOD TOP(:'a))`,
-  RW_TAC fcp_ss [word_1comp_def,n2w_def,ONE_COMP_THM,DIMINDEX_GT_0,TOP]);
+  `!n. ~(n2w n):'a word  = n2w (dimword(:'a) - 1 - n MOD dimword(:'a))`,
+  RW_TAC fcp_ss [word_1comp_def,n2w_def,ONE_COMP_THM,DIMINDEX_GT_0,dimword_def]);
 
 val word_2comp_n2w = store_thm("word_2comp_n2w",
-  `!n. $- (n2w n):'a word  = n2w (TOP(:'a) - n MOD TOP(:'a))`,
+  `!n. $- (n2w n):'a word  = n2w (dimword(:'a) - n MOD dimword(:'a))`,
   SIMP_TAC std_ss [word_2comp_def,n2w_11,w2n_n2w]);
 
 val word_lsb_n2w = store_thm("word_lsb_n2w",
@@ -511,9 +518,9 @@ val word_msb_n2w = store_thm("word_msb_n2w",
 
 val word_msb_n2w_numeric = store_thm(
   "word_msb_n2w_numeric",
-  `word_msb (n2w n : 'a word) = MSB(:'a) <= n MOD TOP(:'a)`,
-  `TOP(:'a) = 2 * MSB(:'a)` by ACCEPT_TAC TOP_IS_TWICE_MSB THEN
-  Q.ABBREV_TAC `WL = TOP (:'a)` THEN
+  `word_msb (n2w n : 'a word) = INT_MIN(:'a) <= n MOD dimword(:'a)`,
+  `dimword(:'a) = 2 * INT_MIN(:'a)` by ACCEPT_TAC dimword_IS_TWICE_INT_MIN THEN
+  Q.ABBREV_TAC `WL = dimword (:'a)` THEN
   `0 < WL` by SRW_TAC [][Abbr`WL`, DIMINDEX_GT_0] THEN
   `(n = (n DIV WL) * WL + n MOD WL) /\ n MOD WL < WL`
      by METIS_TAC [DIVISION] THEN
@@ -524,18 +531,18 @@ val word_msb_n2w_numeric = store_thm(
              DECIDE ``SUC x - x = 1``, EQ_IMP_THM] THEN REPEAT STRIP_TAC
   THENL [
     SPOSE_NOT_THEN ASSUME_TAC THEN
-    `r < MSB(:'a)` by SRW_TAC [ARITH_ss][Abbr`r`] THEN
-    `n DIV MSB(:'a) = 2 * q`
+    `r < INT_MIN(:'a)` by SRW_TAC [ARITH_ss][Abbr`r`] THEN
+    `n DIV INT_MIN(:'a) = 2 * q`
        by (SRW_TAC [][] THEN METIS_TAC [DIV_MULT,
                                         MULT_COMM,
                                         MULT_ASSOC]) THEN
-    METIS_TAC [DECIDE ``~(0n = 1) /\ 0 < 2n``, MOD_EQ_0, MULT_COMM, MSB],
+    METIS_TAC [DECIDE ``~(0n = 1) /\ 0 < 2n``, MOD_EQ_0, MULT_COMM, INT_MIN_def],
 
     MATCH_MP_TAC MOD_UNIQUE THEN
     Q.EXISTS_TAC `q` THEN ASM_SIMP_TAC (srw_ss()) [] THEN
     MATCH_MP_TAC DIV_UNIQUE THEN
-    Q.EXISTS_TAC `r - MSB(:'a)` THEN
-    FULL_SIMP_TAC (srw_ss() ++ ARITH_ss) [MSB]
+    Q.EXISTS_TAC `r - INT_MIN(:'a)` THEN
+    FULL_SIMP_TAC (srw_ss() ++ ARITH_ss) [INT_MIN_def]
   ])
 
 val word_and_n2w = store_thm("word_and_n2w",
@@ -565,7 +572,8 @@ val word_0 = store_thm("word_0",
 
 val word_T = store_thm("word_T",
   `!i. i < ^WL ==> (Tw:'a word) %% i`,
-  SIMP_TAC fcp_ss [word_T_def,n2w_def,ONE_COMP_0_THM,DIMINDEX_GT_0, TOP]);
+  SIMP_TAC fcp_ss [word_T_def,n2w_def,ONE_COMP_0_THM,DIMINDEX_GT_0,
+                   UINT_MAX_def, dimword_def]);
 
 val WORD_ss =
   rewrites [word_1comp_def,word_and_def,word_or_def,word_xor_def,
@@ -659,7 +667,7 @@ val w2w = store_thm("w2w",
     \\ STRIP_ASSUME_TAC EXISTS_HB
     \\ STRIP_ASSUME_TAC (Thm.INST_TYPE [alpha |-> beta] EXISTS_HB)
     \\ RW_TAC (fcp_ss++ARITH_ss) [n2w_def,BIT_def,BITS_COMP_THM2,
-         GSYM BITS_ZERO3, TOP]
+         GSYM BITS_ZERO3, dimword_def]
     \\ Cases_on `i < SUC m`
     \\ ASM_SIMP_TAC (fcp_ss++ARITH_ss) [MIN_DEF,BITS_ZERO]);
 
@@ -722,12 +730,12 @@ val MIN_lem2 = prove(
 val word_bits_w2w = store_thm("word_bits_w2w",
   `!w. (h -- l) (w2w (w:'a word)):'b word =
        w2w ((MIN h (dimindex (:'b) - 1) -- l) w)`,
-  Cases_word \\ SIMP_TAC arith_ss [word_bits_n2w,w2w_def,w2n_n2w,TOP]
+  Cases_word \\ SIMP_TAC arith_ss [word_bits_n2w,w2w_def,w2n_n2w,dimword_def]
     \\ STRIP_ASSUME_TAC EXISTS_HB
     \\ STRIP_ASSUME_TAC (Thm.INST_TYPE [alpha |-> beta] EXISTS_HB)
     \\ ASM_SIMP_TAC arith_ss [n2w_11,GSYM BITS_ZERO3,BITS_COMP_THM2,
          AC MIN_ASSOC MIN_COMM,ONCE_REWRITE_RULE [ADD_COMM] MIN_lem,
-         MIN_lem2,TOP]);
+         MIN_lem2,dimword_def]);
 
 val word_reverse_n2w = store_thm("word_reverse_n2w",
   `!n. word_reverse ((n2w n):'a word) =
@@ -753,7 +761,7 @@ val w2n_w2w = store_thm("w2n_w2w",
     \\ STRIP_ASSUME_TAC EXISTS_HB
     \\ STRIP_ASSUME_TAC (Thm.INST_TYPE [alpha |-> beta] EXISTS_HB)
     \\ ASM_SIMP_TAC arith_ss [BITS_COMP_THM2,w2w_def,word_bits_n2w,
-          REWRITE_RULE [MOD_DIMINDEX,TOP] w2n_n2w]
+          REWRITE_RULE [MOD_DIMINDEX,dimword_def] w2n_n2w]
     \\ RW_TAC arith_ss [MIN_DEF]
     \\ `m' = m` by DECIDE_TAC \\ ASM_REWRITE_TAC []);
 
@@ -764,7 +772,7 @@ val w2w_n2w = store_thm("w2w_n2w",
          else
            n2w (BITS (^WL - 1) 0 n)`,
   RW_TAC arith_ss [MIN_DEF,MOD_DIMINDEX,BITS_COMP_THM2,w2n_n2w,w2w_def,n2w_11,
-                   TOP]);
+                   dimword_def]);
 
 val WORD_EQ = store_thm("WORD_EQ",
   `!v:'a word w. (!x. x < ^WL ==> (word_bit x v = word_bit x w)) = (v = w)`,
@@ -785,7 +793,7 @@ val WORD_BIT_BITS = store_thm("WORD_BIT_BITS",
   `!b w. word_bit b w = ((b -- b) w = 1w)`,
   STRIP_TAC \\ Cases_word
     \\ RW_TAC arith_ss [MIN_DEF,BIT_def,word_bit_n2w,word_bits_n2w,n2w_11,
-         LESS_MOD,lem,lem2,TOP]
+         LESS_MOD,lem,lem2,dimword_def]
     \\ STRIP_ASSUME_TAC EXISTS_HB
     \\ FULL_SIMP_TAC arith_ss [MIN_DEF,GSYM BITS_ZERO3,SUC_SUB1,BITS_COMP_THM2]
     \\ Cases_on `b = 0` \\ FULL_SIMP_TAC arith_ss []
@@ -817,7 +825,7 @@ val WORD_BITS_LT = store_thm("WORD_BITS_LT",
   NTAC 2 STRIP_TAC \\ Cases_word
     \\ STRIP_ASSUME_TAC EXISTS_HB
     \\ RW_TAC arith_ss [word_bits_n2w,w2n_n2w,GSYM BITS_ZERO3,
-         BITS_COMP_THM2,MIN_DEF,BITSLT_THM,TOP]
+         BITS_COMP_THM2,MIN_DEF,BITSLT_THM,dimword_def]
     \\ FULL_SIMP_TAC std_ss []
     << [`SUC m - l <= SUC h - l` by DECIDE_TAC,
      `SUC (l + m) - l <= SUC h - l` by DECIDE_TAC]
@@ -884,7 +892,7 @@ val _ = set_fixity "==" (Infixr 450);
 
 val equiv = ``\x y. x MOD ^top = y MOD ^top``;
 
-val n2w_11' = REWRITE_RULE [TOP] n2w_11
+val n2w_11' = REWRITE_RULE [dimword_def] n2w_11
 val lift_rule = REWRITE_RULE [GSYM n2w_11'] o INST [`wl` |-> `^WL`];
 val LET_RULE = CONV_RULE (DEPTH_CONV pairLib.let_CONV);
 val LET_TAC = CONV_TAC (DEPTH_CONV pairLib.let_CONV);
@@ -943,13 +951,13 @@ val WORD_NEG_mod = LET_RULE (prove(
          (SIMP_RULE bool_ss [GSYM SUC_ONE_ADD,GSYM PRE_SUC_EQ,ZERO_LT_TWOEXP])
     \\ ASM_SIMP_TAC arith_ss [PRE_SUB1]));
 
-val n2w_TOP = prove(
+val n2w_dimword = prove(
   `n2w (2 ** ^WL) = 0w:'a word`,
   ONCE_REWRITE_TAC [GSYM n2w_mod]
-    \\ SIMP_TAC std_ss [DIVMOD_ID,ZERO_MOD,ZERO_LT_TWOEXP,TOP]);
+    \\ SIMP_TAC std_ss [DIVMOD_ID,ZERO_MOD,ZERO_LT_TWOEXP,dimword_def]);
 
 val WORD_ss = rewrites [word_add_n2w,word_mul_n2w,word_sub_def,word_2comp_def,
-  w2n_n2w,n2w_w2n,word_0,n2w_TOP,ZERO_LT_TWOEXP,TOP,
+  w2n_n2w,n2w_w2n,word_0,n2w_dimword,ZERO_LT_TWOEXP,dimword_def,
   LEFT_ADD_DISTRIB,RIGHT_ADD_DISTRIB,
   LEFT_SUB_DISTRIB,RIGHT_SUB_DISTRIB];
 
@@ -1002,7 +1010,7 @@ val WORD_ADD_LINV = store_thm("WORD_ADD_LINV",
          ((REWRITE_RULE [ZERO_LT_TWOEXP] o SPECL [`n`,`2 ** ^WL`]) DA)
     \\ ASM_SIMP_TAC std_ss [MOD_MULT]
     \\ ONCE_REWRITE_TAC [GSYM n2w_mod]
-    \\ ASM_SIMP_TAC arith_ss [GSYM MULT,MOD_EQ_0,ZERO_LT_TWOEXP,word_0,TOP]);
+    \\ ASM_SIMP_TAC arith_ss [GSYM MULT,MOD_EQ_0,ZERO_LT_TWOEXP,word_0,dimword_def]);
 
 val WORD_ADD_RINV = store_thm("WORD_ADD_RINV",
   `!w:'a word. w + $- w = 0w`,
@@ -1048,7 +1056,7 @@ val WORD_NEG = store_thm("WORD_NEG",
   `!w:'a word. $- w = ~w + 1w`,
   REPEAT Cases_word
     \\ ASM_SIMP_TAC (fcp_ss++ARITH_ss) [word_add_n2w,word_2comp_n2w,
-         word_1comp_n2w,lift_rule WORD_NEG_mod,TOP]);
+         word_1comp_n2w,lift_rule WORD_NEG_mod,dimword_def]);
 
 val WORD_NOT = store_thm("WORD_NOT",
   `!w:'a word. ~w = $- w - 1w`,
@@ -1168,11 +1176,11 @@ val WORD_SUB_TRIANGLE = store_thm("WORD_SUB_TRIANGLE",
 
 val WORD_NEG_1 = store_thm("WORD_NEG_1",
   `$- 1w:'a word = Tw:'a word`,
-  REWRITE_TAC [word_T_def,word_2comp_def,w2n_n2w]
-    \\ Cases_on `TOP (:'a) = 1`
+  REWRITE_TAC [word_T_def,word_2comp_def,w2n_n2w,UINT_MAX_def]
+    \\ Cases_on `dimword (:'a) = 1`
     >> ASM_SIMP_TAC arith_ss [n2w_11]
     \\ ASM_SIMP_TAC arith_ss [DECIDE ``0 < x /\ ~(x = 1) ==> 1 < x``,
-         LESS_MOD,ZERO_LT_TWOEXP,TOP]);
+         LESS_MOD,ZERO_LT_TWOEXP,dimword_def]);
 
 val WORD_NOT_0 = save_thm("WORD_NOT_0",
   (GEN_ALL o REWRITE_RULE [WORD_NEG_1,WORD_NEG_0,WORD_SUB_LZERO] o
@@ -1240,7 +1248,7 @@ val ASR_LIMIT = store_thm("ASR_LIMIT",
            (w >> n = if word_msb w then Tw else 0w)`,
   SHIFT_WORD_TAC);
 
-val ASR_TRUE = store_thm("ASR_TRUE",
+val ASR_UINT_MAX = store_thm("ASR_UINT_MAX",
   `!w:'a word n. Tw >> n = Tw`, SHIFT_WORD_TAC);
 
 val LSR_LIMIT = store_thm("LSR_LIMIT",
@@ -1266,14 +1274,14 @@ val SPEC1_RULE = (GEN_ALL o REWRITE_RULE [EXP_1] o
 
 val LSL_ONE = store_thm("LSL_ONE",
   `!w:'a word. w << 1 = w + w`,
-  STRIP_TAC \\ Cases_on_word `w` \\ REWRITE_TAC [word_add_def,w2n_n2w,TOP]
+  STRIP_TAC \\ Cases_on_word `w` \\ REWRITE_TAC [word_add_def,w2n_n2w,dimword_def]
     \\ SHIFT_WORD_TAC \\ Cases_on `1 <= i`
     \\ ASM_SIMP_TAC arith_ss [SPEC1_RULE BIT_SHIFT_THM2,
                               SPEC1_RULE BIT_SHIFT_THM3]
     \\ STRIP_ASSUME_TAC EXISTS_HB \\ POP_ASSUM SUBST_ALL_TAC
     \\ ASM_SIMP_TAC arith_ss [BIT_def,GSYM BITS_ZERO3,BITS_COMP_THM2,MIN_DEF]);
 
-val ROR_TRUE = store_thm("ROR_TRUE",
+val ROR_UINT_MAX = store_thm("ROR_UINT_MAX",
   `!n. Tw #>> n = Tw`, SHIFT_WORD_TAC);
 
 val ROR_ROL = store_thm("ROR_ROL",
@@ -1333,7 +1341,7 @@ val word_lsl_n2w = store_thm("word_lsl_n2w",
     \\ `n = dimindex (:'a) - 1` by DECIDE_TAC
     \\ ONCE_REWRITE_TAC [GSYM n2w_mod]
     \\ ASM_SIMP_TAC (std_ss++numSimps.ARITH_AC_ss) [GSYM EXP,SUB1_SUC,
-         MOD_EQ_0,ZERO_MOD,ZERO_LT_TWOEXP,DIMINDEX_GT_0,TOP]);
+         MOD_EQ_0,ZERO_MOD,ZERO_LT_TWOEXP,DIMINDEX_GT_0,dimword_def]);
 
 val word_lsr_n2w = store_thm("word_lsr_n2w",
   `!w:'a word n. w >>> n = (^HB -- n) w`,
@@ -1342,14 +1350,15 @@ val word_lsr_n2w = store_thm("word_lsr_n2w",
 
 val lem = (GEN_ALL o REWRITE_RULE [MATCH_MP (DECIDE ``0 < n ==> 1 <= n``)
   (SPEC_ALL ZERO_LT_TWOEXP),MULT_LEFT_1] o SPECL [`1`,`2 ** n`]) LESS_MONO_MULT;
-val LSL_TRUE = store_thm("LSL_TRUE",
-  `!n. Tw << n = n2w (TOP(:'a) - 2 ** n):'a word`,
-  RW_TAC arith_ss [n2w_11,word_T_def,word_lsl_n2w,TOP]
+
+val LSL_UINT_MAX = store_thm("LSL_UINT_MAX",
+  `!n. Tw << n = n2w (dimword(:'a) - 2 ** n):'a word`,
+  RW_TAC arith_ss [n2w_11,word_T_def,word_lsl_n2w,dimword_def,UINT_MAX_def]
     \\ FULL_SIMP_TAC arith_ss [NOT_LESS,RIGHT_SUB_DISTRIB]
     \\ `n < ^WL` by DECIDE_TAC \\ IMP_RES_TAC TWOEXP_MONO
-    \\ `2 ** n * ^TOP_ML - 2 ** n =
-          (2 ** n - 1) * ^TOP_ML + (^TOP_ML - 2 ** n)`
-    by (`^TOP_ML <= 2 ** n * ^TOP_ML` by ASM_SIMP_TAC arith_ss [lem]
+    \\ `2 ** n * ^dimword_ML - 2 ** n =
+          (2 ** n - 1) * ^dimword_ML + (^dimword_ML - 2 ** n)`
+    by (`^dimword_ML <= 2 ** n * ^dimword_ML` by ASM_SIMP_TAC arith_ss [lem]
           \\ ASM_SIMP_TAC std_ss [MULT_LEFT_1,RIGHT_SUB_DISTRIB,
                GSYM LESS_EQ_ADD_SUB,LESS_IMP_LESS_OR_EQ,SUB_ADD]
           \\ PROVE_TAC [MULT_COMM])
@@ -1367,7 +1376,7 @@ val word_asr_n2w = prove(
     \\ FULL_SIMP_TAC arith_ss [MIN_DEF]);
 
 val word_asr_n2w = save_thm("word_asr_n2w",
-  REWRITE_RULE [LSL_TRUE] word_asr_n2w);
+  REWRITE_RULE [LSL_UINT_MAX] word_asr_n2w);
 
 val BITS_SUM1 =
   (GEN_ALL o REWRITE_RULE [MULT_LEFT_1] o
@@ -1448,14 +1457,14 @@ val SPEC_LESS_EXP_SUC_MONO = prove(
   SRW_TAC [][DIMINDEX_GT_0])
 
 val SPLIT_2_EXP_WL = prove(
-  `^TOP_ML = ^MSB_ML + ^MSB_ML`,
+  `^dimword_ML = ^INT_MIN_ML + ^INT_MIN_ML`,
   STRIP_ASSUME_TAC EXISTS_HB
     \\ ASM_SIMP_TAC arith_ss [EXP]);
 
 val WORD_NEG_L = store_thm("WORD_NEG_L",
   `$- word_L = word_L`,
-  SRW_TAC [][word_2comp_n2w, word_L_def, LESS_MOD, DIMINDEX_GT_0, TOP, MSB,
-             SUB_RIGHT_EQ, SPLIT_2_EXP_WL])
+  SRW_TAC [][word_2comp_n2w, word_L_def, LESS_MOD, DIMINDEX_GT_0, dimword_def,
+             INT_MIN_def, SUB_RIGHT_EQ, SPLIT_2_EXP_WL])
 
 (* ------------------------------------------------------------------------- *)
 
@@ -1470,20 +1479,20 @@ val SLICE_COMP_MSB = prove(
 
 val MSB_THM1 = prove(
   `!a:'a word. ~(^HB = 0) /\ word_msb a ==>
-        (w2n a = ^MSB_ML + BITS (^HB - 1) 0 (w2n a))`,
+        (w2n a = ^INT_MIN_ML + BITS (^HB - 1) 0 (w2n a))`,
   Cases_word \\ STRIP_ASSUME_TAC EXISTS_HB
     \\ RW_TAC arith_ss [word_msb_n2w,w2n_n2w,GSYM BITS_ZERO3,BITS_COMP_MSB,
-                        TOP]
+                        dimword_def]
     \\ IMP_RES_TAC BIT_SLICE_THM2 \\ POP_ASSUM (SUBST1_TAC o SYM)
     \\ ASM_SIMP_TAC arith_ss [SLICE_COMP_MSB,GSYM SLICE_ZERO_THM]);
 
 val MSB_THM2 = prove(
   `!a:'a word. ~(^HB = 0) /\ word_msb a ==>
-        (w2n ($- a) = ^MSB_ML - BITS (^HB - 1) 0 (w2n a))`,
+        (w2n ($- a) = ^INT_MIN_ML - BITS (^HB - 1) 0 (w2n a))`,
   Cases_word \\ REPEAT STRIP_TAC \\ IMP_RES_TAC MSB_THM1
     \\ STRIP_ASSUME_TAC EXISTS_HB
     \\ FULL_SIMP_TAC arith_ss [word_msb_n2w,word_2comp_n2w,w2n_n2w,
-         BITS_COMP_MSB,GSYM BITS_ZERO3, TOP]
+         BITS_COMP_MSB,GSYM BITS_ZERO3, dimword_def]
     \\ ASM_SIMP_TAC arith_ss [BITS_ZERO3,GSYM ADD1,ADD_MODULUS,MOD_MOD,
          ZERO_LT_TWOEXP,SUB_SUC1]
     \\ REWRITE_TAC [EXP,TIMES2,SUB_PLUS,ADD_SUB]
@@ -1496,7 +1505,7 @@ val MSB_THM3 = prove(
         (w2n a = BITS (^HB - 1) 0 (w2n a))`,
   Cases_word \\ STRIP_ASSUME_TAC EXISTS_HB
     \\ RW_TAC arith_ss [word_msb_n2w,w2n_n2w,GSYM BITS_ZERO3,BITS_COMP_MSB,
-                        TOP]
+                        dimword_def]
     \\ `~(m = 0)` by DECIDE_TAC
     \\ MAP_EVERY IMP_RES_TAC [BIT_SLICE_THM3,SLICE_COMP_MSB]
     \\ POP_ASSUM (SPEC_THEN `n` ASSUME_TAC)
@@ -1505,12 +1514,12 @@ val MSB_THM3 = prove(
 
 val MSB_THM4 = prove(
   `!a:'a word. ~(^HB = 0) /\ ~(a = 0w) /\ ~word_msb a ==>
-       (w2n ($- a) = ^TOP_ML - BITS (^HB - 1) 0 (w2n a)) /\
+       (w2n ($- a) = ^dimword_ML - BITS (^HB - 1) 0 (w2n a)) /\
        ~(BITS (^HB - 1) 0 (w2n a) = 0)`,
   Cases_word \\ REPEAT STRIP_TAC \\ IMP_RES_TAC MSB_THM3
     \\ STRIP_ASSUME_TAC EXISTS_HB
     \\ FULL_SIMP_TAC arith_ss [word_msb_n2w,word_2comp_n2w,w2n_n2w,n2w_11,
-         GSYM BITS_ZERO3,BITS_ZERO2,BITS_COMP_MSB,TOP]
+         GSYM BITS_ZERO3,BITS_ZERO2,BITS_COMP_MSB,dimword_def]
     \\ FULL_SIMP_TAC arith_ss [BITS_COMP_THM2,MIN_DEF]
     \\ `2 ** SUC m - BITS (m - 1) 0 n < 2 ** SUC m`
     by ASM_SIMP_TAC arith_ss [ZERO_LT_TWOEXP]
@@ -1519,14 +1528,14 @@ val MSB_THM4 = prove(
 val HB_0_MSB = prove(
   `!a:'a word. (^HB = 0) /\ word_msb a ==> (a = 1w)`,
   Cases_word \\ STRIP_ASSUME_TAC EXISTS_HB
-    \\ RW_TAC bool_ss [word_msb_n2w,w2n_n2w,n2w_11,BIT_def,SUC_SUB1,TOP]
+    \\ RW_TAC bool_ss [word_msb_n2w,w2n_n2w,n2w_11,BIT_def,SUC_SUB1,dimword_def]
     \\ FULL_SIMP_TAC arith_ss [BITS_ZERO3]);
 
 val HB_0_NOT_MSB = prove(
   `!a:'a word. (^HB = 0) /\ ~word_msb a ==> (a = 0w)`,
   Cases_word \\ STRIP_ASSUME_TAC EXISTS_HB
     \\ RW_TAC fcp_ss [word_msb_n2w,n2w_11,ZERO_MOD,ZERO_LT_TWOEXP,
-         GSYM BITS_ZERO3,TOP]
+         GSYM BITS_ZERO3,dimword_def]
     \\ METIS_TAC [DECIDE ``SUC m <= 1 = (m = 0)``,BIT_def,NOT_BITS2]);
 
 val DIMINDEX_1 = prove(
@@ -1536,27 +1545,27 @@ val DIMINDEX_1 = prove(
 val MSB_THM1b = prove(
   `!a:'a word. (^HB = 0) /\ word_msb a ==> (w2n a = 1)`,
   METIS_TAC [HB_0_MSB,DIMINDEX_1,EXP_1,LESS_MOD,DECIDE ``1 < 2``,w2n_n2w,
-             TOP]);
+             dimword_def]);
 
 val MSB_THM2b = prove(
   `!a:'a word. (^HB = 0) /\ word_msb a ==> (w2n (word_2comp a) = 1)`,
   REPEAT STRIP_TAC \\ MAP_EVERY IMP_RES_TAC [HB_0_MSB,DIMINDEX_1]
-    \\ ASM_SIMP_TAC arith_ss [w2n_n2w,word_2comp_n2w,TOP]);
+    \\ ASM_SIMP_TAC arith_ss [w2n_n2w,word_2comp_n2w,dimword_def]);
 
 val MSB_THM3b = prove(
   `!a:'a word. (^HB = 0) /\ ~word_msb a ==> (w2n a = 0)`,
   REPEAT STRIP_TAC \\ MAP_EVERY IMP_RES_TAC [HB_0_NOT_MSB,DIMINDEX_1]
-    \\ ASM_SIMP_TAC arith_ss [w2n_n2w,TOP]);
+    \\ ASM_SIMP_TAC arith_ss [w2n_n2w,dimword_def]);
 
 val MSB_THM4b = prove(
   `!a:'a word. (^HB = 0) /\ ~word_msb a ==> (w2n (word_2comp a) = 0)`,
   REPEAT STRIP_TAC \\ MAP_EVERY IMP_RES_TAC [HB_0_NOT_MSB,DIMINDEX_1]
-    \\ ASM_SIMP_TAC arith_ss [w2n_n2w,WORD_NEG_0,TOP]);
+    \\ ASM_SIMP_TAC arith_ss [w2n_n2w,WORD_NEG_0,dimword_def]);
 
 (* ------------------------------------------------------------------------- *)
 
-val w2n_mod = PROVE [n2w_w2n,n2w_mod,TOP]
-   ``(w2n (a:'a word) = n) ==> (a = n2w (n MOD ^TOP_ML))``;
+val w2n_mod = PROVE [n2w_w2n,n2w_mod,dimword_def]
+   ``(w2n (a:'a word) = n) ==> (a = n2w (n MOD ^dimword_ML))``;
 
 val BITS_MSB_LT = (GEN_ALL o SIMP_RULE arith_ss [SUB_SUC1] o
   DISCH `~(b = 0)` o SPECL [`b - 1`,`0`,`a`]) BITSLT_THM;
@@ -1591,13 +1600,13 @@ val TWO_COMP_NEG_lem = prove(
        ~(BITS (^WL - 2) 0 (w2n ((n2w n):'a word)) = 0)`,
   REPEAT STRIP_TAC \\ STRIP_ASSUME_TAC EXISTS_HB
     \\ FULL_SIMP_TAC arith_ss [BITS_COMP_THM2,MIN_DEF,GSYM BITS_ZERO3,
-         word_msb_n2w,w2n_n2w,TOP]
+         word_msb_n2w,w2n_n2w,dimword_def]
     \\ IMP_RES_TAC BIT_SLICE_THM2
     \\ RULE_ASSUM_TAC (REWRITE_RULE [GSYM SLICE_ZERO_THM])
     \\ `~(m = 0)` by DECIDE_TAC \\ IMP_RES_TAC SLICE_COMP_MSB
     \\ POP_ASSUM (SPEC_THEN `n` ASSUME_TAC)
     \\ FULL_SIMP_TAC arith_ss [word_L_def,n2w_11,LESS_MOD,
-         SUC_SUB1,SUC_SUB2,TWOEXP_MONO,TOP,MSB]
+         SUC_SUB1,SUC_SUB2,TWOEXP_MONO,dimword_def,INT_MIN_def]
     \\ FULL_SIMP_TAC bool_ss [GSYM BITS_ZERO3,GSYM SLICE_ZERO_THM]
     \\ PROVE_TAC [ADD_0]);
 
@@ -1610,13 +1619,13 @@ val TWO_COMP_NEG = store_thm("TWO_COMP_NEG",
   RW_TAC bool_ss [] << [
     IMP_RES_TAC HB_0_MSB
       \\ ASM_SIMP_TAC arith_ss [word_msb_n2w,word_T_def,WORD_NEG_1,
-           DIMINDEX_GT_0,ONE_COMP_0_THM,TOP],
+           DIMINDEX_GT_0,ONE_COMP_0_THM,UINT_MAX_def,dimword_def],
     ASM_REWRITE_TAC [WORD_NEG_L],
     FULL_SIMP_TAC bool_ss [] \\ Cases_on_word `a`
       \\ MAP_EVERY IMP_RES_TAC [MSB_THM2,w2n_mod,TWO_COMP_NEG_lem]
       \\ STRIP_ASSUME_TAC EXISTS_HB \\ `~(m = 0)` by DECIDE_TAC
       \\ FULL_SIMP_TAC arith_ss [BITS_COMP_THM2,MIN_DEF,BIT_def,
-           word_msb_n2w,w2n_n2w,GSYM BITS_ZERO3,SUC_SUB2,TOP]
+           word_msb_n2w,w2n_n2w,GSYM BITS_ZERO3,SUC_SUB2,dimword_def]
       \\ `2 ** m - BITS (m - 1) 0 n < 2 ** m`
       by ASM_SIMP_TAC arith_ss [ZERO_LT_TWOEXP]
       \\ ASM_SIMP_TAC arith_ss [BITS_THM,SUC_SUB,EXP_1,LESS_DIV_EQ_ZERO]]);
@@ -1637,28 +1646,29 @@ val WORD_0_POS = store_thm("WORD_0_POS",
 
 val WORD_H_POS = store_thm("WORD_H_POS",
   `~word_msb word_H`,
-  `^MSB_ML - 1 < ^MSB_ML` by ASM_SIMP_TAC arith_ss [ZERO_LT_TWOEXP]
+  `^INT_MIN_ML - 1 < ^INT_MIN_ML` by ASM_SIMP_TAC arith_ss [ZERO_LT_TWOEXP]
      \\ ASM_SIMP_TAC bool_ss [word_H_def,word_msb_n2w,BIT_def,BITS_THM,
-          LESS_DIV_EQ_ZERO,ZERO_MOD,ZERO_LT_TWOEXP,MSB] \\ DECIDE_TAC);
+          LESS_DIV_EQ_ZERO,ZERO_MOD,ZERO_LT_TWOEXP,INT_MIN_def,INT_MAX_def]
+     \\ DECIDE_TAC);
 
 val WORD_L_NEG = store_thm("WORD_L_NEG",
   `word_msb word_L`,
-   REWRITE_TAC [word_L_def,word_msb_n2w,BIT_ZERO,BIT_B,MSB]);
+   REWRITE_TAC [word_L_def,word_msb_n2w,BIT_ZERO,BIT_B,INT_MIN_def]);
 
 (* ------------------------------------------------------------------------- *)
 
 val NOT_EQUAL_THEN_NOT =
   PROVE [EQUAL_THEN_SUB_ZERO] ``!a b. ~(a = b) = ~(b - a = 0w)``;
 
-val SUB_EQUAL_WORD_L_MSB = prove(
+val SUB_EQUAL_WORD_L_INT_MIN = prove(
   `!a:'a word b:'a word. ~(^HB = 0) /\ (a - b = word_L) ==>
       ~(word_msb a = word_msb b)`,
   RW_TAC bool_ss [WORD_EQ_SUB_RADD] \\ STRIP_ASSUME_TAC EXISTS_HB
     \\ `~(m = 0)` by DECIDE_TAC \\ Cases_on_word `b`
-    \\ ASM_REWRITE_TAC [word_msb_n2w,word_L_def,SUC_SUB1,MSB]
+    \\ ASM_REWRITE_TAC [word_msb_n2w,word_L_def,SUC_SUB1,INT_MIN_def]
     \\ SUBST1_TAC ((SYM o SPEC `n`) n2w_mod)
     \\ ASM_REWRITE_TAC [word_msb_n2w,word_add_n2w,SUC_SUB1,
-         GSYM BITS_ZERO3,GSYM SLICE_ZERO_THM,TOP]
+         GSYM BITS_ZERO3,GSYM SLICE_ZERO_THM,dimword_def]
     \\ `SLICE m 0 n = SLICE m m n + SLICE (m - 1) 0 n`
     by METIS_TAC [SLICE_COMP_MSB,SUC_SUB2]
     \\ Cases_on `BIT m n`
@@ -1674,14 +1684,14 @@ val LEM1_TAC =
     \\ GEN_REWRITE_TAC (RATOR_CONV o ONCE_DEPTH_CONV)
          empty_rewrites [GSYM WORD_NEG_SUB]
     \\ IMP_RES_TAC NOT_EQUAL_THEN_NOT \\ Cases_on `b - a = word_L`
-    \\ PROVE_TAC [SUB_EQUAL_WORD_L_MSB,TWO_COMP_POS_NEG];
+    \\ PROVE_TAC [SUB_EQUAL_WORD_L_INT_MIN,TWO_COMP_POS_NEG];
 
 val LEM2_TAC =
   REPEAT STRIP_TAC \\ MAP_EVERY Cases_on [`word_msb a`,`word_msb b`]
     \\ MAP_EVERY IMP_RES_TAC [MSB_THM1b,MSB_THM2b,MSB_THM3b,MSB_THM4b]
     \\ ASM_SIMP_TAC arith_ss [word_lt,word_gt,word_le,word_ge,word_sub_def,
          word_add_def,word_add_n2w,word_msb_n2w,n2w_11,BITS_ZERO2,BIT_def,
-         TOP]
+         dimword_def]
     \\ ASM_SIMP_TAC arith_ss [BITS_ZERO3]
     \\ PROVE_TAC [w2n_11];
 
@@ -1709,7 +1719,7 @@ val start_tac =
   REWRITE_TAC [word_sub_def,word_add_def] \\ RW_TAC bool_ss [word_msb_n2w]
     \\ POP_ASSUM MP_TAC \\ Cases_on `w2n a < w2n b`
     \\ ASM_REWRITE_TAC [] \\ IMP_RES_TAC MSB_THM1
-    \\ `w2n ($- b) = ^MSB_ML - BITS (^HB - 1) 0 (w2n b)`
+    \\ `w2n ($- b) = ^INT_MIN_ML - BITS (^HB - 1) 0 (w2n b)`
           by IMP_RES_TAC MSB_THM2
     \\ ABBREV_TAC `x = BITS (^HB - 1) 0 (w2n a)`
     \\ ABBREV_TAC `y = BITS (^HB - 1) 0 (w2n b)`
@@ -1737,8 +1747,8 @@ val WORD_LT_lem2 = prove(
     \\ ONCE_REWRITE_TAC [DECIDE (Term `!a b c. (a:num) + b + c = a + c + b`)]
     \\ PAT_ASSUM `x + y < x + z` (ASSUME_TAC o (MATCH_MP LESS_ADD2))
     \\ IMP_RES_TAC LESS_ADD_1
-    \\ `y < ^MSB_ML` by METIS_TAC [BITS_MSB_LT]
-    \\ `p + 1 <= ^MSB_ML` by DECIDE_TAC
+    \\ `y < ^INT_MIN_ML` by METIS_TAC [BITS_MSB_LT]
+    \\ `p + 1 <= ^INT_MIN_ML` by DECIDE_TAC
     \\ ASM_SIMP_TAC arith_ss [SUB_LEFT_ADD] \\ IMP_RES_TAC LESS_EQUAL_ADD
     \\ ASM_SIMP_TAC std_ss [TIMES2,DECIDE ``x + (y + p) = x + p + y:num``,
          DECIDE ``a + b + c - (c + b) = a:num``]
@@ -1747,7 +1757,7 @@ val WORD_LT_lem2 = prove(
     \\ numLib.REDUCE_TAC);
 
 val w2n_0 =
-  SIMP_CONV arith_ss [w2n_n2w,ZERO_MOD,ZERO_LT_TWOEXP,TOP] ``w2n 0w``;
+  SIMP_CONV arith_ss [w2n_n2w,ZERO_MOD,ZERO_LT_TWOEXP,dimword_def] ``w2n 0w``;
 
 val start_tac = REWRITE_TAC [word_sub_def,word_add_def]
     \\ NTAC 2 STRIP_TAC
@@ -1758,12 +1768,12 @@ val start_tac = REWRITE_TAC [word_sub_def,word_add_def]
     \\ POP_ASSUM MP_TAC
     \\ Cases_on `w2n a < w2n b` \\ ASM_REWRITE_TAC []
     \\ IMP_RES_TAC MSB_THM3
-    \\ `w2n ($- b) = ^TOP_ML - BITS (^HB - 1) 0 (w2n b)`
+    \\ `w2n ($- b) = ^dimword_ML - BITS (^HB - 1) 0 (w2n b)`
           by IMP_RES_TAC MSB_THM4
     \\ ABBREV_TAC `x = BITS (^HB - 1) 0 (w2n a)`
     \\ ABBREV_TAC `y = BITS (^HB - 1) 0 (w2n b)`
-    \\ `y <= ^MSB_ML` by METIS_TAC [BITS_MSB_LTEQ]
-    \\ `y <= ^TOP_ML` by METIS_TAC [SPEC_LESS_EXP_SUC_MONO,
+    \\ `y <= ^INT_MIN_ML` by METIS_TAC [BITS_MSB_LTEQ]
+    \\ `y <= ^dimword_ML` by METIS_TAC [SPEC_LESS_EXP_SUC_MONO,
                                     LESS_IMP_LESS_OR_EQ,LESS_EQ_TRANS]
     \\ FULL_SIMP_TAC bool_ss [NOT_LESS,GSYM LESS_EQ_ADD_SUB]
     \\ ONCE_REWRITE_TAC [ADD_COMM];
@@ -1771,8 +1781,8 @@ val start_tac = REWRITE_TAC [word_sub_def,word_add_def]
 val WORD_LT_lem3 = prove(
   `!a:'a word b. ~(^HB = 0) /\ ~word_msb a /\ ~word_msb b /\
          word_msb (a - b) ==> w2n a < w2n b`,
-  start_tac \\ `x < ^MSB_ML` by METIS_TAC [BITS_MSB_LT]
-    \\ `x - y < ^MSB_ML` by DECIDE_TAC
+  start_tac \\ `x < ^INT_MIN_ML` by METIS_TAC [BITS_MSB_LT]
+    \\ `x - y < ^INT_MIN_ML` by DECIDE_TAC
     \\ STRIP_ASSUME_TAC EXISTS_HB
     \\ FULL_SIMP_TAC bool_ss [BIT_def,BITS_THM,SUC_SUB,EXP_1,
          LESS_EQ_ADD_SUB,EXP,DIV_MULT,SUC_SUB1]
@@ -1782,10 +1792,10 @@ val WORD_LT_lem4 = prove(
   `!a:'a word b. ~(^HB = 0) /\ ~word_msb a /\ ~word_msb b /\
         ~word_msb (a - b) ==> ~(w2n a < w2n b)`,
   start_tac
-    \\ `y <= ^MSB_ML + x` by DECIDE_TAC
+    \\ `y <= ^INT_MIN_ML + x` by DECIDE_TAC
     \\ ASM_SIMP_TAC bool_ss [SPLIT_2_EXP_WL,GSYM ADD_ASSOC,LESS_EQ_ADD_SUB]
     \\ IMP_RES_TAC LESS_IMP_LESS_OR_EQ
-    \\ `^MSB_ML - (y - x) < ^MSB_ML` by DECIDE_TAC
+    \\ `^INT_MIN_ML - (y - x) < ^INT_MIN_ML` by DECIDE_TAC
     \\ STRIP_ASSUME_TAC EXISTS_HB
     \\ FULL_SIMP_TAC bool_ss [LESS_EQ_ADD_SUB2,DIV_MULT_1,BIT_def,
          BITS_THM,SUC_SUB,EXP_1]
@@ -1818,10 +1828,10 @@ val WORD_GE = save_thm("WORD_GE",
   ``a:'a word >= b``);
 
 val w2n_2comp = prove(
-  `!a:'a word. w2n ($- a) = if a = 0w then 0 else ^TOP_ML - w2n a`,
+  `!a:'a word. w2n ($- a) = if a = 0w then 0 else ^dimword_ML - w2n a`,
   RW_TAC bool_ss [WORD_NEG_0,w2n_0] \\ Cases_on_word `a`
-    \\ FULL_SIMP_TAC bool_ss [GSYM w2n_11,w2n_0,w2n_n2w,word_2comp_n2w,TOP]
-    \\ `^TOP_ML - n MOD ^TOP_ML < ^TOP_ML`
+    \\ FULL_SIMP_TAC bool_ss [GSYM w2n_11,w2n_0,w2n_n2w,word_2comp_n2w,dimword_def]
+    \\ `^dimword_ML - n MOD ^dimword_ML < ^dimword_ML`
           by ASM_SIMP_TAC arith_ss [ZERO_LT_TWOEXP]
     \\ ASM_SIMP_TAC bool_ss [LESS_MOD]);
 
@@ -1829,7 +1839,7 @@ val WORD_LO = store_thm("WORD_LO",
   `!a b. a <+ b = w2n a < w2n b`,
   RW_TAC bool_ss [word_lo] \\ Cases_on `b = 0w`
     \\ ASM_SIMP_TAC arith_ss [w2n_2comp,w2n_0,GSYM LESS_EQ_ADD_SUB,
-         REWRITE_RULE [TOP]
+         REWRITE_RULE [dimword_def]
                       (MATCH_MP LESS_IMP_LESS_OR_EQ (SPEC `b` w2n_lt))]
     \\ Cases_on `a = b` >> ASM_SIMP_TAC arith_ss [BIT_B]
     \\ Cases_on `w2n a < w2n b` \\ ASM_REWRITE_TAC []
@@ -1837,13 +1847,14 @@ val WORD_LO = store_thm("WORD_LO",
     \\ RULE_ASSUM_TAC (REWRITE_RULE [GSYM w2n_11,w2n_0,w2n_n2w]) << [
       IMP_RES_TAC LESS_IMP_LESS_OR_EQ
         \\ `~(w2n b - w2n a = 0)` by DECIDE_TAC
-        \\ POP_ASSUM (fn th => `^TOP_ML - (w2n b - w2n a) < ^TOP_ML`
+        \\ POP_ASSUM (fn th => `^dimword_ML - (w2n b - w2n a) < ^dimword_ML`
                                    by SIMP_TAC arith_ss [th,ZERO_LT_TWOEXP])
         \\ ASM_SIMP_TAC arith_ss [GSYM SUB_SUB,BIT_def,BITS_THM,SUC_SUB,
              EXP_1,LESS_DIV_EQ_ZERO],
       RULE_ASSUM_TAC (REWRITE_RULE [NOT_LESS])
-        \\ ASSUME_TAC (REWRITE_RULE [TOP] (SPEC `a` w2n_lt))
-        \\ `w2n a - w2n b < ^TOP_ML` by ASM_SIMP_TAC arith_ss [ZERO_LT_TWOEXP]
+        \\ ASSUME_TAC (REWRITE_RULE [dimword_def] (SPEC `a` w2n_lt))
+        \\ `w2n a - w2n b < ^dimword_ML`
+        by ASM_SIMP_TAC arith_ss [ZERO_LT_TWOEXP]
         \\ ASM_SIMP_TAC bool_ss [LESS_EQ_ADD_SUB,BIT_def,BITS_THM,SUC_SUB,
              EXP_1,DIV_MULT_1]
         \\ numLib.REDUCE_TAC]);
@@ -2042,14 +2053,15 @@ val WORD_NOT_LOWER_EQ = store_thm("WORD_NOT_LOWER_EQ",
 
 (* ------------------------------------------------------------------------- *)
 
-val w2n_word_L = SIMP_CONV arith_ss
-  [word_L_def,w2n_n2w,LESS_MOD,SPEC_LESS_EXP_SUC_MONO,MSB,TOP] ``w2n word_L``;
+val w2n_word_L = SIMP_CONV arith_ss [word_L_def,w2n_n2w,LESS_MOD,
+  SPEC_LESS_EXP_SUC_MONO,INT_MIN_def,dimword_def] ``w2n word_L``;
 
 val w2n_word_H = prove(
-  `w2n (word_H:'a word) = ^MSB_ML - 1`,
-  `^MSB_ML - 1 < ^MSB_ML` by SIMP_TAC arith_ss [ZERO_LT_TWOEXP]
+  `w2n (word_H:'a word) = ^INT_MIN_ML - 1`,
+  `^INT_MIN_ML - 1 < ^INT_MIN_ML` by SIMP_TAC arith_ss [ZERO_LT_TWOEXP]
     \\ ASSUME_TAC SPEC_LESS_EXP_SUC_MONO \\ IMP_RES_TAC LESS_TRANS
-    \\ ASM_SIMP_TAC arith_ss [word_H_def,w2n_n2w,LESS_MOD,MSB,TOP]);
+    \\ ASM_SIMP_TAC arith_ss [word_H_def,w2n_n2w,LESS_MOD,
+         INT_MAX_def,INT_MIN_def,dimword_def]);
 
 val WORD_L_PLUS_H = store_thm("WORD_L_PLUS_H",
   `word_L + word_H = word_T`,
@@ -2063,7 +2075,7 @@ fun bound_tac th1 th2 =
     \\ Cases_on `^HB = 0`
     >> (IMP_RES_TAC th1 \\ ASM_SIMP_TAC arith_ss [])
     \\ Cases_on_word `a`
-    \\ FULL_SIMP_TAC bool_ss [w2n_n2w,word_msb_n2w,TOP]
+    \\ FULL_SIMP_TAC bool_ss [w2n_n2w,word_msb_n2w,dimword_def]
     \\ MAP_EVERY IMP_RES_TAC [th2,SLICE_COMP_MSB]
     \\ POP_ASSUM (SPEC_THEN `n` ASSUME_TAC)
     \\ STRIP_ASSUME_TAC EXISTS_HB
@@ -2093,47 +2105,47 @@ val WORD_L_LESS_H = store_thm("WORD_L_LESS_H",
 
 val WORD_ss = rewrites
   [WORD_LT,WORD_GT,WORD_LE,WORD_GE,WORD_LS,WORD_HI,WORD_LO,WORD_HS,
-   word_msb_n2w,w2n_n2w,TOP];
+   word_msb_n2w,w2n_n2w,dimword_def];
 
 val ORDER_WORD_TAC =
   SIMP_TAC (bool_ss++boolSimps.LET_ss++WORD_ss) [] \\ DECIDE_TAC;
 
 val word_lt_n2w = store_thm("word_lt_n2w",
   `!a b. (n2w a):'a word < n2w b =
-            let sa = BIT ^HB a and sb = BIT ^HB b
-            in
-              (sa = sb) /\ a MOD TOP(:'a) < b MOD TOP(:'a) \/ sa /\ ~sb`,
+          let sa = BIT ^HB a and sb = BIT ^HB b
+          in
+            (sa = sb) /\ a MOD dimword(:'a) < b MOD dimword(:'a) \/ sa /\ ~sb`,
   ORDER_WORD_TAC);
 
 val word_gt_n2w = store_thm("word_gt_n2w",
   `!a b. (n2w a):'a word > n2w b = let sa = BIT ^HB a and sb = BIT ^HB b in
-    (sa = sb) /\ a MOD TOP(:'a) > b MOD TOP(:'a) \/ ~sa /\ sb`,
+    (sa = sb) /\ a MOD dimword(:'a) > b MOD dimword(:'a) \/ ~sa /\ sb`,
   ORDER_WORD_TAC);
 
 val word_le_n2w = store_thm("word_le_n2w",
   `!a b. (n2w a):'a word <= n2w b = let sa = BIT ^HB a and sb = BIT ^HB b in
-    (sa = sb) /\ a MOD TOP(:'a) <= b MOD TOP(:'a) \/ sa /\ ~sb`,
+    (sa = sb) /\ a MOD dimword(:'a) <= b MOD dimword(:'a) \/ sa /\ ~sb`,
   ORDER_WORD_TAC);
 
 val word_ge_n2w = store_thm("word_ge_n2w",
   `!a b. (n2w a):'a word >= n2w b = let sa = BIT ^HB a and sb = BIT ^HB b in
-    (sa = sb) /\ a MOD TOP(:'a) >= b MOD TOP(:'a) \/ ~sa /\ sb`,
+    (sa = sb) /\ a MOD dimword(:'a) >= b MOD dimword(:'a) \/ ~sa /\ sb`,
   ORDER_WORD_TAC);
 
 val word_ls_n2w = store_thm("word_ls_n2w",
-  `!a b. (n2w a):'a word <=+ n2w b = a MOD TOP(:'a) <= b MOD TOP(:'a)`,
+  `!a b. (n2w a):'a word <=+ n2w b = a MOD dimword(:'a) <= b MOD dimword(:'a)`,
   ORDER_WORD_TAC);
 
 val word_hi_n2w = store_thm("word_hi_n2w",
-  `!a b. (n2w a):'a word >+ n2w b = a MOD TOP(:'a) > b MOD TOP(:'a)`,
+  `!a b. (n2w a):'a word >+ n2w b = a MOD dimword(:'a) > b MOD dimword(:'a)`,
   ORDER_WORD_TAC);
 
 val word_lo_n2w = store_thm("word_lo_n2w",
-  `!a b. (n2w a):'a word <+ n2w b = a MOD TOP(:'a) < b MOD TOP(:'a)`,
+  `!a b. (n2w a):'a word <+ n2w b = a MOD dimword(:'a) < b MOD dimword(:'a)`,
   ORDER_WORD_TAC);
 
 val word_hs_n2w = store_thm("word_hs_n2w",
-  `!a b. (n2w a):'a word >=+ n2w b = a MOD TOP(:'a) >= b MOD TOP(:'a)`,
+  `!a b. (n2w a):'a word >=+ n2w b = a MOD dimword(:'a) >= b MOD dimword(:'a)`,
   ORDER_WORD_TAC);
 
 (* ------------------------------------------------------------------------- *)
@@ -2144,26 +2156,26 @@ val WORD_PRED_THM = store_thm("WORD_PRED_THM",
   `!m:'a word. ~(m = 0w) ==> w2n (m - 1w) < w2n m`,
   Cases_word \\ Cases_on `n` \\  RW_TAC arith_ss [w2n_n2w]
     \\ POP_ASSUM MP_TAC \\ SIMP_TAC arith_ss [ZERO_MOD,ZERO_LT_TWOEXP,
-         ADD1,WORD_ADD_SUB,GSYM word_add_n2w,w2n_n2w,n2w_11,TOP,
-         (SIMP_RULE arith_ss [ZERO_LT_TWOEXP] o SPEC `^TOP_ML`) MOD_ADD_1]);
+         ADD1,WORD_ADD_SUB,GSYM word_add_n2w,w2n_n2w,n2w_11,dimword_def,
+         (SIMP_RULE arith_ss [ZERO_LT_TWOEXP] o SPEC `^dimword_ML`) MOD_ADD_1]);
 
 (* ------------------------------------------------------------------------- *)
 (* Create a few word sizes                                                   *)
 (* ------------------------------------------------------------------------- *)
 
-val sizes = [2, 3, 4, 5, 6, 7, 8, 12, 16, 20, 24, 28, 32, 64];
+val sizes = [2, 3, 4, 5, 6, 7, 8, 12, 16, 20, 24, 28, 30, 32, 64];
 
 fun mk_word_size n =
   let val (_, _, dimindex_thm) = fcpLib.mk_index_type n
       val sn = Int.toString n
       val ityp = mk_type("i"^sn, [])
       val TYPE = mk_type("cart", [bool, ityp])
-      val msb = save_thm("msb_" ^ sn,
+      val INT_MIN = save_thm("INT_MIN_" ^ sn,
                   (SIMP_RULE std_ss [dimindex_thm] o
-                   Thm.INST_TYPE [``:'a`` |-> ityp]) MSB)
-      val top = save_thm("top_" ^ sn,
-                  (SIMP_RULE std_ss [msb] o
-                   Thm.INST_TYPE [``:'a`` |-> ityp]) TOP_IS_TWICE_MSB)
+                   Thm.INST_TYPE [``:'a`` |-> ityp]) INT_MIN_def)
+      val dimword = save_thm("dimword_" ^ sn,
+                  (SIMP_RULE std_ss [INT_MIN] o
+                   Thm.INST_TYPE [``:'a`` |-> ityp]) dimword_IS_TWICE_INT_MIN)
   in
     type_abbrev("word"^sn, TYPE)
   end;
